compiler/src/compiler/RegRename.v
@@ -122,53 +122,6 @@ Module map.
     - eapply H0.
   Qed.
 
-  Definition map_all_values_V0{K V1 V2: Type}{M1: map.map K V1}{M2: map.map K V2}
-             (f: V1 -> option V2)(m1: M1)(keys: list K): option M2 :=
-    bind_opt values2 <- List.option_all
-                           (List.map (fun k => bind_opt v1 <- map.get m1 k; f v1) keys);
-    map.of_list_zip keys values2.
-
-  Definition map_all_values{K V1 V2: Type}{M1: map.map K V1}{M2: map.map K V2}
-             (f: V1 -> option V2)(m1: M1): list K -> option M2 :=
-    fix rec keys :=
-      match keys with
-      | nil => Some map.empty
-      | k :: ks =>
-        match map.get m1 k with
-        | Some v1 => match f v1 with
-                     | Some v2 => match rec ks with
-                                  | Some res => Some (map.put res k v2)
-                                  | None => None
-                                  end
-                     | None => None
-                     end
-        | None => None
-        end
-      end.
-
-  Lemma get_map_all_values{K V1 V2: Type}{M1: map.map K V1}{M2: map.map K V2}
-        (keqb: K -> K -> bool) {keqb_spec: EqDecider keqb}
-        {OK1: map.ok M1} {OK2: map.ok M2} (f: V1 -> option V2):
-    forall (keys: list K) (m1: M1) (m2: M2) (k: K) (v1: V1),
-      map_all_values f m1 keys = Some m2 ->
-      In k keys ->
-      map.get m1 k = Some v1 ->
-      exists v2, f v1 = Some v2 /\ map.get m2 k = Some v2.
-  Proof.
-    induction keys; intros.
-    - simpl in *. contradiction.
-    - simpl in *.
-      destruct H0.
-      + subst. rewrite H1 in H. simp.
-        rewrite map.get_put_same. eauto.
-      + simp.
-        rewrite map.get_put_dec.
-        * destr (keqb a k).
-          { (* Automation? clear keqb keqb_spec OK1 OK2 IHkeys. firstorder congruence. (* <- fails *) *)
-            subst. eexists. split; [|reflexivity]. congruence. }
-          { eauto. }
-  Qed.
-
 End map.
 
 Section RegAlloc.
